Make progress with word_bignumScript

compiler/backend/bignum/word_bignumScript.sml
@@ -17,6 +17,39 @@ val _ = Datatype `
        | Loop prog
        | Continue`
 
+(* syntax helper funs *)
+
+val Skip_tm = ``Skip:'a word_bignum$prog``
+val Continue_tm = ``Continue:'a word_bignum$prog``
+
+local val s = HolKernel.syntax_fns1 "word_bignum" in
+  val (Loop_tm,mk_Loop,dest_Loop,is_Loop) = s "Loop"
+end
+local val s = HolKernel.syntax_fns2 "word_bignum" in
+  val (Assign_tm,mk_Assign,dest_Assign,is_Assign) = s "Assign"
+  val (Seq_tm,mk_Seq,dest_Seq,is_Seq) = s "Seq"
+end
+local val s = HolKernel.syntax_fns3 "word_bignum" in
+  val (Load_tm,mk_Load,dest_Load,is_Load) = s "Load"
+  val (Store_tm,mk_Store,dest_Store,is_Store) = s "Store"
+end
+
+local val s = HolKernel.syntax_fns1 "asm" in
+  val (Imm_tm,mk_Imm,dest_Imm,is_Imm) = s "Imm"
+  val (Reg_tm,mk_Reg,dest_Reg,is_Reg) = s "Reg"
+end
+
+val If_pat = ``word_bignum$If c r (ri:'a reg_imm) p1 p2``
+fun dest_If tm = let
+  val i = fst (match_term If_pat tm)
+  val ts = helperLib.list_dest dest_comb If_pat
+  in (subst i (el 2 ts),
+      subst i (el 3 ts),
+      subst i (el 4 ts),
+      subst i (el 5 ts),
+      subst i (el 6 ts)) end
+fun mk_If (c,r,ri,p1,p2) = ``word_bignum$If ^c ^r ^ri ^p1 ^p2``;
+
 (* semantics of the little language *)
 
 val _ = Datatype `
@@ -24,14 +57,31 @@ val _ = Datatype `
            ; arrays : address -> ('a word) list
            |>`
 
-val eval_exp_pre_def = Define `
-  (eval_exp_pre s (Const w) <=> T) /\
-  (eval_exp_pre s (Var v) <=> v IN FDOM s.regs)`
-
 val eval_exp_def = Define `
   eval_exp s (Const w) = w /\
   eval_exp s (Var v) = s.regs ' v /\
-  eval_exp s (Op Add [x1;x2]) = eval_exp s x1 + eval_exp s x2`
+  eval_exp s (Op Add [x1;x2]) = eval_exp s x1 + eval_exp s x2 /\
+  eval_exp s (Op Sub [x1;x2]) = eval_exp s x1 - eval_exp s x2 /\
+  eval_exp s (Op And [x1;x2]) = word_and (eval_exp s x1) (eval_exp s x2) /\
+  eval_exp s (Op Or [x1;x2]) = word_or (eval_exp s x1) (eval_exp s x2) /\
+  eval_exp s (Op Xor [x1;x2]) = word_xor (eval_exp s x1) (eval_exp s x2) /\
+  eval_exp s (Shift sh x (Nat n)) = THE (word_sh sh (eval_exp s x) n)`
+
+val eval_exp_pre_def = Define `
+  (eval_exp_pre s (Const w) <=> T) /\
+  (eval_exp_pre s (Var v) <=> v IN FDOM s.regs) /\
+  (eval_exp_pre s (Op _ [x;y]) <=> eval_exp_pre s x /\ eval_exp_pre s y) /\
+  (eval_exp_pre s (Shift sh x (Nat n)) <=> eval_exp_pre s x /\
+                                           IS_SOME (word_sh sh (eval_exp s x) n)) /\
+  (eval_exp_pre s _ <=> F)`
+
+val eval_ri_pre_def = Define `
+  (eval_ri_pre s (Reg r) <=> eval_exp_pre (s:'a state) ((Var r):'a wordLang$exp)) /\
+  (eval_ri_pre s (Imm (w:'a word)) <=> T)`;
+
+val eval_ri_def = Define `
+  eval_ri s (Reg r) = eval_exp s (Var r) /\
+  eval_ri s (Imm w) = w`
 
 val (eval_rules,eval_ind,raw_eval_cases) = Hol_reln `
   (!s. Eval s Skip (INR (s:'a state))) /\
@@ -42,6 +92,11 @@ val (eval_rules,eval_ind,raw_eval_cases) = Hol_reln `
   (!s1 s2 s3 p1 p2.
      Eval s1 p1 (INR s2) /\ Eval s2 p2 s3 ==>
      Eval s1 (Seq p1 p2) s3) /\
+  (!s1 c r ri p1 p2 s2.
+     r IN FDOM s.regs /\ eval_ri_pre s ri /\
+     Eval s1 (if word_cmp c (eval_exp s (Var r)) (eval_ri s ri)
+              then p1 else p2) s2 ==>
+     Eval s1 (If c r ri p1 p2) s2) /\
   (!s1 p s2.
      Eval s1 p (INR s2) ==>
      Eval s1 (Loop p) (INR s2)) /\
@@ -52,9 +107,10 @@ val (eval_rules,eval_ind,raw_eval_cases) = Hol_reln `
 val eval_cases =
   map (SIMP_CONV (srw_ss()) [Once raw_eval_cases])
     [``Eval s1 Skip s2``,
+     ``Eval s1 Continue s2``,
      ``Eval s1 (Seq p1 p2) s2``,
      ``Eval s1 (Assign n x) s2``,
-     ``Eval s1 Continue s2``,
+     ``Eval s1 (If c r ri p1 p2) s2``,
      ``Eval s1 (Loop p) s2``] |> LIST_CONJ;
 
 (* correctenss judgement *)
@@ -74,7 +130,7 @@ val COMB_def = Define `
                  let (s2,b3) = f s1 in (s2,b2 /\ b3)`;
 
 val Corr_Seq = prove(
-  ``Corr p1 (TERM g) /\ Corr p2 f ==>
+  ``Corr p1 (TERM g) ==> Corr p2 f ==>
     Corr (Seq p1 p2) (COMB g f)``,
   fs [Corr_def,TERM_def,COMB_def,eval_cases] \\ rw []
   \\ rpt (pop_assum mp_tac)
@@ -83,7 +139,7 @@ val Corr_Seq = prove(
   \\ metis_tac [SND,FST,PAIR]);
 
 val Corr_Continue = prove(
-  ``Corr Continue (\s. (INL s,b))``,
+  ``Corr Continue (\s. (INL s,T))``,
   fs [Corr_def,eval_cases]);
 
 val Corr_Assign = prove(
@@ -91,6 +147,15 @@ val Corr_Assign = prove(
       (TERM (\s. (s with regs := s.regs |+ (n,eval_exp s x),
                   eval_exp_pre s x)))``,
   fs [Corr_def,eval_cases,TERM_def]);
+
+val Corr_If = prove(
+  ``Corr p1 f1 /\ Corr p2 f2 ==>
+    Corr (If c r ri p1 p2)
+         (\s. (I ## (\b. b /\ r IN FDOM s.regs /\ eval_ri_pre s ri))
+              (if word_cmp c (eval_exp s (Var r)) (eval_ri s ri)
+               then f1 s else f2 s))``,
+  fs [Corr_def,eval_cases] \\ rw [] \\ fs []
+  \\ asm_exists_tac \\ fs [] \\ rw [] \\ fs []);
 
 val LOOP_def = Define `
   LOOP f = \s. (SHORT_TAILREC f s, SHORT_TAILREC_PRE f s)`;
@@ -108,5 +173,177 @@ val Corr_Loop = prove(
   \\ Cases_on `f s` \\ fs []
   \\ Cases_on `q` \\ fs []
   \\ asm_exists_tac \\ fs []);
+
+val Corr_STRENGTHEN = prove(
+  ``Corr p f ==>
+    !f'.
+      (!s. FST (f' s) = FST (f s)) /\
+      (!s. SND (f' s) ==> SND (f s)) ==>
+      Corr p f'``,
+  fs [Corr_def] \\ metis_tac []);
+
+val Corr_STRENGTHEN_TERM = prove(
+  ``Corr p (TERM f) ==>
+    !f'.
+      (!s. FST (f' s) = FST (f s)) /\
+      (!s. SND (f' s) ==> SND (f s)) ==>
+      Corr p (TERM f')``,
+  fs [Corr_def,TERM_def]
+  \\ CONV_TAC (DEPTH_CONV PairRules.PBETA_CONV) \\ fs []);
+
+(* examples *)
+
+fun tailrec_define name tm =
+  tailrecLib.tailrec_define_from_step name tm NONE;
+
+val (foo_def, _,foo_pre_def, _) =
+  tailrec_define "foo" ``
+    (\(r8,r10).
+      let r10 = r10 - 8w in
+      let r8 = r8 + r10 in
+        if r8 <+ r10 then (INR r8,T) else (INL (r8,r10),T))
+    :('a word) # ('a word) -> (((('a word) # ('a word)) + ('a word)) # bool)``
+
+(* generate deep embeddings *)
+
+fun my_dest_let tm = let
+  val (x,y) = pairSyntax.dest_anylet tm
+  in if length x = 1 then (hd x,y) else fail() end
+
+local
+  val word_ty = ``:'a word``
+in
+  fun dest_reg v = let
+    val (n,ty) = dest_var v
+    val _ = ty = word_ty orelse fail()
+    val n = String.substring(n,1,String.size(n)-1) |> string_to_int
+    val n = numSyntax.term_of_int n
+    in n end handle Subscript => fail()
+end;
+
+val binops = [(word_add_def,``asm$Add``),
+              (word_sub_def,``asm$Sub``),
+              (word_and_def,``asm$And``),
+              (word_xor_def,``asm$Xor``),
+              (word_or_def, ``asm$Or``)]
+  |> map (fn (x,y) => (x |> SPEC_ALL |> concl |> dest_eq |> fst, y))
+
+fun get_exp x =
+  (* Var *) let
+  val n = dest_reg x
+  in wordLangSyntax.mk_Var n end handle HOL_ERR _ =>
+  (* Const *) let
+  val _ = wordsSyntax.dest_n2w x
+  in wordLangSyntax.mk_Const x end handle HOL_ERR _ =>
+  (* Op *) let
+  val (_,name) = first (fn (pat,_) => can (match_term pat) x) binops
+  val x1 = get_exp (x |> rator |> rand)
+  val x2 = get_exp (x |> rand)
+  in wordLangSyntax.mk_Op(name,listSyntax.mk_list([x1,x2],type_of x1)) end
+
+val cmps = [(word_lo_def,``asm$Lower``),
+            (word_lt_def,``asm$Less``),
+            (GSYM w2n_11,``asm$Equal``)]
+  |> map (fn (x,y) => (x |> SPEC_ALL |> concl |> dest_eq |> fst, y))
+
+fun dest_reg_imm ri =
+  mk_Reg (dest_reg ri) handle HOL_ERR _ =>
+  if can wordsSyntax.dest_n2w ri then mk_Imm ri else fail()
+
+fun get_guard b = (* Op *) let
+  val (_,name) = first (fn (pat,_) => can (match_term pat) b) cmps
+  val x1 = dest_reg (b |> rator |> rand)
+  val x2 = dest_reg_imm (b |> rand)
+  in (name,x1,x2) end handle HOL_ERR _ => let
+  val _ = can (match_term ``(w && n2w n) = 0w:'a word``) b orelse fail()
+  val x1 = b |> rator |> rand |> rator |> rand
+  val x2 = b |> rator |> rand |> rand
+  in (``asm$Test``,dest_reg x1,dest_reg_imm x2) end
+
+fun get_prog tm =
+  (* return *)
+  if is_var tm then Skip_tm else
+  if pairSyntax.is_pair tm then Skip_tm else
+  (* Assign *) let
+  val ((v,x),rest) = my_dest_let tm
+  val n = dest_reg v
+  val e = get_exp x
+  val r = get_prog rest
+  in mk_Seq(mk_Assign(n,e),r) end handle HOL_ERR _ => let
+  val (b,t1,t2) = dest_cond tm
+  val (x1,x2,x3) = get_guard b
+  in mk_If(x1,x2,x3,get_prog t1,get_prog t2) end handle HOL_ERR _ =>
+  if is_const (rator tm) andalso (is_var (rand tm) orelse is_pair (rand tm))
+  then Continue_tm
+  else fail()
+
+fun get_full_prog tm = mk_Loop(get_prog tm);
+
+(*
+val tm = foo_def |> SPEC_ALL |> concl |> rand
+*)
+
+(* derive Corr thm from AST *)
+
+(*
+  val tm = foo_def |> SPEC_ALL |> concl |> rand
+  val tm = get_full_prog tm
+*)
+
+fun get_pat thm = thm |> SPEC_ALL |> UNDISCH_ALL |> concl |> rator |> rand;
+
+fun get_corr tm =
+  if tm = Skip_tm then Corr_Skip else
+  if tm = Continue_tm then Corr_Continue else let
+  val i = fst (match_term (get_pat Corr_Assign) tm)
+  in REWRITE_RULE [eval_exp_def,eval_exp_pre_def] (INST i Corr_Assign) end
+  handle HOL_ERR _ => let
+  val (p1,p2) = dest_Seq tm
+  val th1 = get_corr p1
+  val th2 = get_corr p2
+  in MATCH_MP (MATCH_MP Corr_Seq th1) th2 end
+  handle HOL_ERR _ => let
+  val i = fst (match_term (get_pat Corr_Loop) tm)
+  val th = get_corr (tm |> rand)
+  in MATCH_MP Corr_Loop th end handle HOL_ERR _ => let
+  val i = fst (match_term (get_pat Corr_If) tm)
+  val p1 = get_corr (tm |> rator |> rand)
+  val p2 = get_corr (tm |> rand)
+  val th = REWRITE_RULE [eval_exp_def,eval_exp_pre_def,asmSemTheory.word_cmp_def,
+             eval_ri_pre_def,eval_ri_def] (INST i Corr_If)
+  in MATCH_MP th (CONJ p1 p2) end
+
+(*
+  get_corr tm
+*)
+
+val foo_corr = get_corr tm
+
+val foo_raw_def = Define `
+  foo_raw = ^(foo_corr |> concl |> rand |> rand)`
+
+val foo_corr = foo_corr |> REWRITE_RULE [GSYM foo_raw_def]
+
+val v = mk_var("foo_new",type_of (foo_raw_def |> concl |> rator |> rand))
+
+val foo_new_def = Define `
+  ^v = \s.
+    (let r8 = foo (s.regs ' 8, s.regs ' 10) in
+     let s1 = FST (foo_raw s) in
+       s with regs := (s.regs |++ [(8,r8); (10,s1.regs ' 10)]),
+     8 IN FDOM s.regs /\
+     10 IN FDOM s.regs /\
+     foo_pre (s.regs ' 8, s.regs ' 10))`
+
+val foo_corr_lemma =
+  MATCH_MP Corr_STRENGTHEN_TERM foo_corr
+  |> SPEC (foo_new_def |> concl |> rator |> rand)
+
+val lemma = prove(``^(foo_corr_lemma |> concl |> dest_imp |> fst)``,
+  reverse conj_tac
+  \\ fs [foo_new_def,fetch "-" "foo_pre",foo_raw_def,LOOP_def]
+  \\ cheat);
+
+val corr_foo_new = MP foo_corr_lemma lemma |> REWRITE_RULE [foo_new_def];
 
 val _ = export_theory();
